theories/zoo_saturn/ws_queue_2.v
@@ -43,24 +43,32 @@ Section ws_queue_2_G.
   Definition ws_queue_2_model t vs : iProp Σ :=
     ∃ slots,
     ws_queue_1_model t (#@{location} <$> slots) ∗
-    [∗ list] slot; v ∈ slots; vs, slot ↦ᵣ v.
+    [∗ list] slot; v ∈ slots; vs, slot ↦ᵣ□ v.
   #[local] Instance : CustomIpatFormat "model" :=
     "(
-      %slots{} &
+      %slots_vs{} &
       Hmodel{_{}} &
-      Hslots{}
+      Hslots_vs{}
     )".
 
-  Definition ws_queue_2_owner :=
-    ws_queue_1_owner.
+  Definition ws_queue_2_owner t ws : iProp Σ :=
+    ∃ slots,
+    ws_queue_1_owner t (#@{location} <$> slots) ∗
+    [∗ list] slot; v ∈ slots; ws, slot ↦ᵣ□ v.
+  #[local] Instance : CustomIpatFormat "owner" :=
+    "(
+      %slots_ws{} &
+      Howner{_{}} &
+      Hslots_ws{}
+    )".
 
   #[global] Instance ws_queue_2_model_timeless t vs :
     Timeless (ws_queue_2_model t vs).
   Proof.
     apply _.
   Qed.
-  #[global] Instance ws_queue_2_owner_timeless t :
-    Timeless (ws_queue_2_owner t).
+  #[global] Instance ws_queue_2_owner_timeless t ws :
+    Timeless (ws_queue_2_owner t ws).
   Proof.
     apply _.
   Qed.
@@ -79,12 +87,34 @@ Section ws_queue_2_G.
     iApply (ws_queue_1_model_exclusive with "Hmodel_1 Hmodel_2").
   Qed.
 
-  Lemma ws_queue_2_owner_exclusive t :
-    ws_queue_2_owner t -∗
-    ws_queue_2_owner t -∗
+  Lemma ws_queue_2_owner_exclusive t ws1 ws2 :
+    ws_queue_2_owner t ws1 -∗
+    ws_queue_2_owner t ws2 -∗
     False.
   Proof.
-    apply ws_queue_1_owner_exclusive.
+    iIntros "(:owner =1) (:owner =2)".
+    iApply (ws_queue_1_owner_exclusive with "Howner_1 Howner_2").
+  Qed.
+  Lemma ws_queue_2_owner_model t ws vs :
+    ws_queue_2_owner t ws -∗
+    ws_queue_2_model t vs -∗
+    ⌜vs `suffix_of` ws⌝.
+  Proof.
+    iIntros "(:owner =1) (:model)".
+    iDestruct (ws_queue_1_owner_model with "Howner_1 Hmodel") as %(slots & ->)%suffix_fmap; last congruence.
+    iDestruct (big_sepL2_app_inv_l with "Hslots_ws1") as "(%ws1 & %vs_ & -> & _ & Hslots_vs_)".
+
+    iAssert ⌜vs = vs_⌝%I as %<-.
+    { rewrite list_eq_Forall2.
+      iApply big_sepL2_Forall2.
+      iDestruct (big_sepL2_retract_l with "Hslots_vs") as "(% & Hvs)".
+      iDestruct (big_sepL2_retract_l with "Hslots_vs_") as "(% & Hvs_)".
+      iDestruct (big_sepL2_sepL_2 with "Hvs Hvs_") as "H"; first congruence.
+      iApply (big_sepL2_impl with "H"). iIntros "!> %i %v %v_ _ _ ((%slot1 & %Hslots_vs_lookup_1 & Hl1) & (%slot2 & %Hslots_vs_lookup_2 & Hl2))". simplify.
+      iApply (pointsto_agree with "Hl1 Hl2").
+    }
+
+    iExists ws1. iSteps.
   Qed.
 
   Lemma ws_queue_2_create_spec ι :
@@ -96,20 +126,20 @@ Section ws_queue_2_G.
       RET t;
       ws_queue_2_inv t ι ∗
       ws_queue_2_model t [] ∗
-      ws_queue_2_owner t
+      ws_queue_2_owner t []
     }}}.
   Proof.
     iIntros "%Φ _ HΦ".
 
     wp_apply (ws_queue_1_create_spec with "[//]") as (t) "(#Hinv & Hmodel & Howner)".
 
-    iSteps. iExists []. iSteps.
+    iSteps. iExists []. iSteps. iExists []. iSteps.
   Qed.
 
-  Lemma ws_queue_2_push_spec t ι v :
+  Lemma ws_queue_2_push_spec t ι ws v :
     <<<
       ws_queue_2_inv t ι ∗
-      ws_queue_2_owner t
+      ws_queue_2_owner t ws
     | ∀∀ vs,
       ws_queue_2_model t vs
     >>>
@@ -117,19 +147,20 @@ Section ws_queue_2_G.
     <<<
       ws_queue_2_model t (vs ++ [v])
     | RET ();
-      ws_queue_2_owner t
+      ws_queue_2_owner t (vs ++ [v])
     >>>.
   Proof.
-    iIntros "%Φ (#Hinv & Howner) HΦ".
+    iIntros "%Φ (#Hinv & (:owner)) HΦ".
 
     wp_rec.
     wp_ref slot as "Hslot".
+    iMod (pointsto_persist with "Hslot") as "#Hslot".
 
     awp_apply (ws_queue_1_push_spec with "[$Hinv $Howner]").
     iApply (aacc_aupd_commit with "HΦ"); first done. iIntros "%vs (:model)".
     iAaccIntro with "Hmodel"; iIntros "Hmodel !>"; first iSteps.
-    iDestruct (big_sepL2_snoc_2 with "Hslots Hslot") as "Hslots".
-    rewrite -fmap_snoc. iFrameSteps.
+    iDestruct (big_sepL2_snoc_2 with "Hslots_vs Hslot") as "Hslots".
+    rewrite -fmap_snoc. iSteps.
   Qed.
 
   Lemma ws_queue_2_steal_spec t ι :
@@ -152,48 +183,50 @@ Section ws_queue_2_G.
     awp_smart_apply (ws_queue_1_steal_spec with "Hinv").
     iApply (aacc_aupd_commit with "HΦ"); first done. iIntros "%vs (:model)".
     iAaccIntro with "Hmodel"; iIntros "Hmodel !>"; first iSteps.
-    destruct slots as [| slot slots], vs as [| v vs] => //.
+    destruct slots_vs as [| slot slots_vs], vs as [| v vs] => //.
     all: iFrameSteps.
   Qed.
 
-  Lemma ws_queue_2_pop_spec t ι :
+  Lemma ws_queue_2_pop_spec t ι ws :
     <<<
       ws_queue_2_inv t ι ∗
-      ws_queue_2_owner t
+      ws_queue_2_owner t ws
     | ∀∀ vs,
       ws_queue_2_model t vs
     >>>
       ws_queue_2_pop t @ ↑ι
     <<<
-      ∃∃ o,
+      ∃∃ o ws,
       match o with
       | None =>
           ⌜vs = []⌝ ∗
+          ⌜ws = []⌝ ∗
           ws_queue_2_model t []
       | Some v =>
           ∃ vs',
           ⌜vs = vs' ++ [v]⌝ ∗
+          ⌜ws = vs'⌝ ∗
           ws_queue_2_model t vs'
       end
     | RET o;
-      ws_queue_2_owner t
+      ws_queue_2_owner t ws
     >>>.
   Proof.
-    iIntros "%Φ (#Hinv & Howner) HΦ".
+    iIntros "%Φ (#Hinv & (:owner)) HΦ".
 
     wp_rec.
 
     awp_smart_apply (ws_queue_1_pop_spec with "[$Hinv $Howner]").
     iApply (aacc_aupd_commit with "HΦ"); first done. iIntros "%vs (:model)".
-    iAaccIntro with "Hmodel"; first iSteps. iIntros ([𝑠𝑙𝑜𝑡 |]).
-    - iIntros "(%𝑠𝑙𝑜𝑡s & %Hslots & Hmodel) !>".
-      apply fmap_snoc_inv in Hslots as (slots' & slot & -> & -> & ->).
-      iDestruct (big_sepL2_snoc_inv_l with "Hslots") as "(%vs' & %v & -> & Hslots & Hslot)".
+    iAaccIntro with "Hmodel"; first iSteps. iIntros ([𝑠𝑙𝑜𝑡 |] slots_ws').
+    - iIntros "(%𝑠𝑙𝑜𝑡s & %Hslots_vs & <- & Hmodel) !>".
+      apply fmap_snoc_inv in Hslots_vs as (slots_vs' & slot & -> & -> & ->).
+      iDestruct (big_sepL2_snoc_inv_l with "Hslots_vs") as "(%vs' & %v & -> & #Hslots_vs' & #Hslot)".
       iExists (Some v). iFrameSteps.
-    - iIntros "(%Hslots & Hmodel) !>".
-      apply fmap_nil_inv in Hslots as ->.
-      iDestruct (big_sepL2_nil_inv_l with "Hslots") as %->.
-      iExists None. iFrameSteps.
+    - iIntros "(%Hslots_vs & -> & Hmodel) !>".
+      apply fmap_nil_inv in Hslots_vs as ->.
+      iDestruct (big_sepL2_nil_inv_l with "Hslots_vs") as %->.
+      iExists None. iFrameSteps. iExists []. iSteps.
   Qed.
 End ws_queue_2_G.
 
